#+TAGS: IDENTITY(i) INVERSE(n)
* Sum

** Group axioms

*** Identity

**** Definition
- [ ] a + 0 = a
- [ ] 0 + a = a
- [ ] a + 0 = 0 + a


**** Variation
- [ ] (a + b) + 0 = a + b
- [ ] x + (y + 0) = x + y

**** Composition
- [ ] n = (n + 0) + 0

*** Inverse

**** Definition
- [ ] a + -a = 0
- [ ] -a + a = 0

**** Variation
- [ ] (a + b) + -(a + b) = 0

*** Associativity
Should introduce shortcut

**** Definition
- [ ] a + (b + c) = (a + b) + c

*** Compositions
- [ ] a + b + -b + -a = 0
- [ ]

** Commutativity
Should introduce shortcut

*** Definition
- [ ] a + b = b + a

*** Compositions
- [ ] a + b + c = c + a + b

** Left cancellation
a + x = b + x <=> a = b

** Inverse of inverse
-(-a) = a

** Uniqueness of inverse
a + -a = 0 ^ a + -a' = 0 => -a = -a'

* Product

** Group axioms
Same as for sum.

** Distributivity

*** Definition
- [ ] a(b + c) = ab + bc
- [ ] (a + b)c = ac + bc

** Compositions
- [ ] 0x = 0
<=>
0x + 0x = 0 + 0x
0x = (0 + 0)x = 0x + 0x = 0 + 0x = 0x
- [ ] 2x = x + x

** (-a)x = -(ax)
proof:
ax + (-a)x = ax + -(ax)
ax + (-a)x = (a + -a)x = 0x = 0 = ax + -ax

*** Applications

- [ ] (-1)x = -x
- [ ] (-a)(-b) = ab
(-a)(-b) = -(a(-b)) = -(-(ab)) = ab
